yet another update

src/Choreography.v
@@ -3,6 +3,11 @@ From Qoreo Require Expr.
 
 From Stdlib Require Import Structures.Equalities.
 From Stdlib Require Import Program.Equality.
+From Stdlib Require Import Logic.
+From Stdlib Require Import Logic.Decidable.
+From Stdlib Require Import Bool.Bool.
+From Stdlib Require Import Setoid.
+
 
 Module Insn.
     Inductive t : Type :=
@@ -54,23 +59,152 @@ Module Insn.
 
     Definition bind_eq  (Ax : bindt) (By: bindt) : Prop := (fst Ax) = (fst By) /\ (snd Ax) = (snd By).
 
-    Lemma nbeq : forall Ax By, ((fst Ax) <> (fst By) \/ (snd Ax) <> (snd By)) -> ~(bind_eq Ax By).
+    Lemma beq : forall Ax By, (bind_eq Ax By) <-> ((fst Ax) = (fst By) /\ (snd Ax) = (snd By)).
+      Proof.
+        intros.
+        split.
+        { intros. unfold bind_eq in H. auto. }
+        { intros. unfold bind_eq. auto. }
+      Qed.
+        
+    Lemma nbeq : forall Ax By, ((fst Ax) <> (fst By) \/ (snd Ax) <> (snd By)) <-> ~(bind_eq Ax By).
     Proof.
-      intros. unfold bind_eq. tauto.
+      intros.
+      split.
+      { intros. unfold bind_eq. tauto. }
+      { intros. unfold bind_eq in H. tauto. }
+    Qed.
+
+    Lemma nbeqlr : forall Ax By, ((fst Ax) <> (fst By) \/ (snd Ax) <> (snd By)) -> ~(bind_eq Ax By).
+    Proof.
+      intros.
+      pose proof (nbeq Ax By) as Hnbeq.
+      destruct Hnbeq as [HnbeqA _].
+      apply HnbeqA.
+      auto.
+    Qed.
+           
+    Lemma bind_eq_symmetric : forall Ax By, bind_eq Ax By -> bind_eq By Ax.
+    Proof.
+      intros (A,x) (B,y) H.
+      unfold bind_eq.
+      unfold bind_eq in H.
+      intuition.
+    Qed.
+           
+    Lemma bind_neq_symmetric : forall Ax By, ~ bind_eq Ax By -> ~ bind_eq By Ax.
+    Proof.
+      intros (A,x) (B,y) H.
+      unfold bind_eq.
+      unfold bind_eq in H.
+      intuition.
     Qed.
     
     Definition bind_eq_dec  (Ax : bindt) (By: bindt) : {bind_eq Ax By} + {~(bind_eq Ax By)} :=
       match ((Actor.eq_dec (fst Ax) (fst By)), (Var.eq_dec (snd Ax) (snd By))) with
       | (left pt1, left pt2) => left (conj pt1 pt2)
-      | (right pt1, _) => right (nbeq Ax By (or_introl pt1))
-      | (_, right pt2) => right (nbeq Ax By (or_intror pt2))
-      end.
-    
-    Definition bind_eqb (Ax : bindt) (By: bindt) : bool :=
-      match (bool_of_sumbool (bind_eq_dec Ax By)) with
-      | exist _ x _ => x
+      | (right pt1, _) => right (nbeqlr Ax By (or_introl pt1))
+      | (_, right pt2) => right (nbeqlr Ax By (or_intror pt2))
       end.
 
+    (* Unwieldy but leaving as advanced technical example. *)
+    (* Definition bind_eqb (Ax : bindt) (By: bindt) : bool :=
+       match (bool_of_sumbool (bind_eq_dec Ax By)) with
+       | exist _ x _ => x
+       end. *)
+
+    Definition bind_eqb (Ax : bindt) (By: bindt) : bool :=
+      if (bind_eq_dec Ax By) then true else false.
+
+    Lemma bind_eqb_true : forall Ax By, 
+      bind_eqb Ax By = true <-> bind_eq Ax By.
+    Proof.
+      intros.
+      split.
+      {
+        intros.
+        pose proof (beq Ax By) as Hbeq.
+        destruct Hbeq as [HbeqA HbeqB].
+        apply HbeqB.
+        unfold bind_eqb in H.
+        (* NOTE destruction of dependent type with desired spec! *)
+        destruct (bind_eq_dec Ax By) in H.
+        {
+          specialize (HbeqA b).
+          auto.
+        }
+        { discriminate. }
+      }
+      {
+        intros.
+        unfold bind_eqb.
+        destruct (bind_eq_dec Ax By).
+        { reflexivity. }
+        { contradiction. }
+      }
+    Qed.
+
+    Lemma bind_eqb_false : forall Ax By, 
+      bind_eqb Ax By = false <-> ~ bind_eq Ax By.
+    Proof.
+      intros.
+      split.
+      {
+        intros.
+        pose proof (nbeq Ax By) as Hnbeq.
+        destruct Hnbeq as [HnbeqA HnbeqB].
+        apply HnbeqA.
+        unfold bind_eqb in H.
+        (* NOTE destruction of dependent type with desired spec! *)
+        destruct (bind_eq_dec Ax By) in H.
+        { discriminate. }
+        {
+          apply HnbeqB in n.
+          auto.
+        }
+      }
+      {
+        intros.
+        unfold bind_eqb.
+        destruct (bind_eq_dec Ax By).
+        { contradiction. }
+        { reflexivity. }
+      }
+    Qed.
+
+    Lemma bind_eqb_symmetric : forall Ax By, bind_eqb Ax By = bind_eqb By Ax.
+    Proof.
+      intros.
+
+      pose proof (bind_eq_symmetric By Ax) as Hbeqs.
+      pose proof (bind_neq_symmetric By Ax) as Hbneqs.
+      
+      destruct (bind_eqb By Ax) eqn:Heqb.
+      {
+        pose proof (bind_eqb_true Ax By) as HbeqABt.
+        destruct HbeqABt as [HbeqABtA HbeqABtB].
+        pose proof (bind_eqb_true By Ax) as HbeqBAt.
+        destruct HbeqBAt as [HbeqBAtA HbeqBAtB].
+        
+        apply HbeqABtB.
+        specialize (HbeqBAtA Heqb).
+        specialize (Hbeqs HbeqBAtA).
+        auto.
+      }
+      {        
+        pose proof (bind_eqb_false Ax By) as HbeqABf.
+        destruct HbeqABf as [HbeqABfA HbeqABfB].
+        pose proof (bind_eqb_false By Ax) as HbeqBAf.
+        destruct HbeqBAf as [HbeqBAfA HbeqBAfB].
+        
+        apply HbeqABfB.        
+        specialize (HbeqBAfA Heqb).
+        specialize (Hbneqs HbeqBAfA).
+        auto.
+      }
+
+    Qed.
+    
     Definition rebound_in (A : Actor.t) (x : Var.t) (I : t) : bool :=
       match I with
       | Send B1 e B2 y => bind_eqb (A,x) (B2,y)    
@@ -92,17 +226,7 @@ Module Choreography.
       | [] => []
       | (Ins :: C') => (Insn.subst A x v Ins)::(if (Insn.rebound_in A x Ins)
                                                 then C' else (subst A x v C')) 
-      end. 
-
-    (* Fixpoint subst (A : Actor.t) (x : Var.t) (v : Expr.t) (C : t) : t :=
-      match C with
-      | [] => []
-      | (Ins :: C') =>
-          if (List.existsb (Insn.bind_eqb (A,x)) (Insn.bindings (Ins))) then
-            (Insn.subst A x v Ins)::C'
-          else
-            (Insn.subst A x v Ins)::(subst A x v C') 
-      end.*)
+      end.
 End Choreography.
 
 Module Label.
@@ -215,14 +339,13 @@ Inductive WellTyped : ChorEnv.t Expr.typ -> ChorEnv.t Expr.typ -> ChorEnv.t nat 
     WellTyped G (ChorEnv.add B y Expr.QUBIT (ChorEnv.add A x Expr.QUBIT D)) T C ->
 
     ~ Var.Map.In x (ChorEnv.find A D) ->
-    ~ Var.Map.In y (ChorEnv.find A D) ->
+    ~ Var.Map.In y (ChorEnv.find B D) ->
 
     WellTyped G D T ((Insn.EPR A x B y)::C)
 
 | Send : forall DeltaA1 DeltaA2 ThetaA1 ThetaA2 G D T A e tau B y C,
     A <> B ->
     Expr.WellTyped (ChorEnv.find A G) DeltaA1 ThetaA1 e (Expr.BANG tau) ->
-    (* ces changed ThetaA1 to ThetaA2 below-- correct? fix other cases? *)
     WellTyped (ChorEnv.add B y tau G) (Actor.Map.add A DeltaA2 D) (Actor.Map.add A ThetaA2 T) C ->
 
     Var.Map.Partition (ChorEnv.find A D) DeltaA1 DeltaA2 ->
@@ -233,7 +356,7 @@ Inductive WellTyped : ChorEnv.t Expr.typ -> ChorEnv.t Expr.typ -> ChorEnv.t nat 
 | LetBang : forall DeltaA1 DeltaA2 ThetaA1 ThetaA2 G D T A x e tau C,
 
     Expr.WellTyped (ChorEnv.find A G) DeltaA1 ThetaA1 e (Expr.BANG tau) ->
-    WellTyped (ChorEnv.add A x tau G) (Actor.Map.add A DeltaA2 D) (Actor.Map.add A ThetaA1 T) C ->
+    WellTyped (ChorEnv.add A x tau G) (Actor.Map.add A DeltaA2 D) (Actor.Map.add A ThetaA2 T) C ->
 
     Var.Map.Partition (ChorEnv.find A D) DeltaA1 DeltaA2 ->
     Var.Map.Partition (ChorEnv.find A T) ThetaA1 ThetaA2 ->
@@ -243,18 +366,21 @@ Inductive WellTyped : ChorEnv.t Expr.typ -> ChorEnv.t Expr.typ -> ChorEnv.t nat 
 | LetIn : forall DeltaA1 DeltaA2 ThetaA1 ThetaA2 G D T A x e tau C,
 
     Expr.WellTyped (ChorEnv.find A G) DeltaA1 ThetaA1 e tau ->
-    WellTyped G (Actor.Map.add A (Var.Map.add x tau DeltaA2) D) (Actor.Map.add A ThetaA1 T) C ->
+    WellTyped G (Actor.Map.add A (Var.Map.add x tau DeltaA2) D) (Actor.Map.add A ThetaA2 T) C ->
 
     Var.Map.Partition (ChorEnv.find A D) DeltaA1 DeltaA2 ->
     Var.Map.Partition (ChorEnv.find A T) ThetaA1 ThetaA2 ->
     ~ Var.Map.In x DeltaA2 ->
 
+    (* Leaving this here as the analogue of shadowing requirement in Expr.WellTyped, that
+       I argue is not necessary. *)
+    (* WellTyped (Actor.Map.add A (Var.Map.remove x (ChorEnv.find A G)) G) D T ((Insn.Let A x e)::C) *)
     WellTyped G D T ((Insn.Let A x e)::C)
 
 | LetPair: forall DeltaA1 DeltaA2 ThetaA1 ThetaA2 G D T A x1 x2 tau1 tau2 e C,
 
     Expr.WellTyped (ChorEnv.find A G) DeltaA1 ThetaA1 e (Expr.Tensor tau1 tau2) ->
-    WellTyped G (Actor.Map.add A (Var.Map.add x1 tau1 (Var.Map.add x2 tau2 DeltaA2)) D) (Actor.Map.add A ThetaA1 T) C ->
+    WellTyped G (Actor.Map.add A (Var.Map.add x1 tau1 (Var.Map.add x2 tau2 DeltaA2)) D) (Actor.Map.add A ThetaA2 T) C ->
 
     Var.Map.Partition (ChorEnv.find A D) DeltaA1 DeltaA2 ->
     Var.Map.Partition (ChorEnv.find A T) ThetaA1 ThetaA2 ->
@@ -264,20 +390,285 @@ Inductive WellTyped : ChorEnv.t Expr.typ -> ChorEnv.t Expr.typ -> ChorEnv.t nat 
     WellTyped G D T ((Insn.LetPair A x1 x2 e)::C)
 .
 
-
 From Stdlib Require Import Morphisms. (* for Proper *)
 
 Global Instance WellTypedProper : Proper (ChorEnv.Equal ==> ChorEnv.Equal ==> ChorEnv.Equal ==> eq ==> iff) WellTyped.
 Admitted.
 
-Lemma extension : forall A G x (tau : Expr.typ),
-    ChorEnv.MapsTo A x tau G <-> Var.Map.MapsTo x tau (ChorEnv.find A G).
+(* Helpful Lemmas about binding equality based on Insn.beq *)
+Lemma nbeq : forall A B x y,
+    A <> B -> ~ ((Insn.bind_eqb (A,x) (B,y)) = true).
 Proof.
-  intros A G x tau.
-  split.
-  auto.
+  intros.
+  pose proof (Insn.bind_eqb_false (A,x) (B,y)).
+  destruct H0.
+  pose proof (not_true_iff_false (Insn.bind_eqb (A, x) (B, y))).
+  destruct H2.
+  apply H3.
+  apply H1.
+  pose proof (Insn.nbeq (A,x) (B,y)).
+  destruct H4.
+  apply H4.
+  simpl.
   auto.
 Qed.
+
+Lemma beq : forall A B x y,
+    Insn.bind_eqb (A, x) (B, y) = true <-> (A = B /\ x = y).
+Proof.
+  intros.
+  pose proof (Insn.bind_eqb_true (A, x) (B, y)).
+  rewrite -> (Insn.beq (A, x) (B, y)) in H.
+  simpl in H.
+  auto.
+Qed.
+
+Lemma nbeqeq : forall A x y,
+    Insn.bind_eqb (A, x) (A, y) = false ->
+    x <> y.
+Proof.
+  intros.  
+  pose proof (Insn.bind_eqb_false (A, x) (A, y)).
+  destruct H0.
+  specialize (H0 H).
+  rewrite -> (Insn.beq (A, x) (A, y)) in H0.
+  simpl in H0.
+  auto.
+Qed.
+
+Lemma beqeq : forall A x y,
+    Insn.bind_eqb (A, x) (A, y) = true ->
+    x = y.
+Proof.
+  intros.
+  pose proof (Insn.bind_eqb_true (A, x) (A, y)).
+  destruct H0.
+  specialize (H0 H).
+  rewrite -> (Insn.beq (A, x) (A, y)) in H0.
+  simpl in H0.
+  destruct H0.
+  auto.
+Qed.  
+
+(* A slew of Lemmas for manipulating environment mappings. *)
+
+(* START Jennifer to address with map tactics. *)
+
+Lemma nin_dj : forall  {X : Type} x (M1 : Var.Map.t X) M2,
+    Var.Map.Properties.Disjoint M1 M2 ->
+    Var.Map.In x M2 ->
+    ~ Var.Map.In x M1.
+Proof.
+Admitted.
+
+Lemma partitionm_refl : forall {X : Type} (M : Var.Map.t X) M1 M2,
+    Var.Map.Partition M M1 M2 -> Var.Map.Partition M M2 M1.
+Proof.
+Admitted.
+    
+Lemma add_empty_delta : forall A x tau (D : ChorEnv.t Expr.typ),
+    ~ Actor.Map.Empty (ChorEnv.add A x tau D).
+Proof.
+Admitted.
+
+Lemma find_add : forall {X : Type} A M (CE : ChorEnv.t X),
+    (ChorEnv.find A (Actor.Map.add A M CE)) = M.
+Proof.
+Admitted.
+
+Lemma find_ab_neq1 : forall {X : Type} A B x tau (CE : ChorEnv.t X),
+    A <> B ->
+    (ChorEnv.find A (ChorEnv.add B x tau CE)) = (ChorEnv.find A CE).
+Proof.
+Admitted.
+
+Lemma find_ab_neq2 : forall {X : Type} A B M (CE : ChorEnv.t X),
+    A <> B ->
+    (ChorEnv.find A (Actor.Map.add B M CE)) = (ChorEnv.find A CE).
+Proof.
+Admitted.
+
+Lemma find_nbeq : forall (CE : ChorEnv.t Expr.typ) A x B y tau,
+    Insn.bind_eqb (A, x) (B, y) = false -> 
+    ~ Var.Map.In x (ChorEnv.find A CE) ->
+    ~ Var.Map.In x (ChorEnv.find A (ChorEnv.add B y tau CE)).
+Proof.
+Admitted.
+
+Lemma add_find : forall (CE : ChorEnv.t Expr.typ) A x tau,
+    (ChorEnv.find A (ChorEnv.add A x tau CE)) = (Var.Map.add x tau (ChorEnv.find A CE)).
+Proof.
+Admitted.
+
+Lemma add_remove : forall (CE : ChorEnv.t Expr.typ) M A x tau,
+    Var.Map.MapsTo x tau M ->
+    (ChorEnv.add A x tau (Actor.Map.add A (Var.Map.remove x M) CE)) =
+      (Actor.Map.add A M CE).
+Proof.
+Admitted.
+
+Lemma nin_remove : forall (M : Var.Map.t Expr.typ) x,
+    ~ (Var.Map.In x (Var.Map.remove x M)).
+Proof.
+Admitted.
+
+Lemma partition_remove : forall (Delta : Var.Map.t Expr.typ) Delta1 Delta2 x tau,
+    Var.Map.Partition (Var.Map.add x tau Delta) Delta1 Delta2 ->
+    ~ Var.Map.In x Delta ->
+    ~ Var.Map.In x Delta1 ->
+    Var.Map.Partition Delta Delta1 (Var.Map.remove x Delta2).
+Proof.
+Admitted.
+
+Lemma remove_add : forall x tau (Delta1 : Var.Map.t Expr.typ) Delta2,
+    ~ Var.Map.In x Delta1 ->
+    Delta2 = Var.Map.add x tau Delta1 ->
+    (Var.Map.remove x Delta2) = Delta1.
+Proof.
+Admitted.
+
+Lemma addadd1 : forall A (D : ChorEnv.t Expr.typ) Delta x tau,
+    (Actor.Map.add A Delta (ChorEnv.add A x tau D)) = (Actor.Map.add A Delta D).
+Proof.
+Admitted.
+
+Lemma addadd2 : forall {X : Type} A (T : ChorEnv.t X) Theta1 Theta2,
+    (Actor.Map.add A Theta1 (Actor.Map.add A Theta2 T)) = (Actor.Map.add A Theta1 T).
+Proof.
+Admitted.
+
+Lemma addadd3 :  forall (CE : ChorEnv.t Expr.typ) A x tau B M,
+  A <> B -> 
+  Actor.Map.add B M (ChorEnv.add A x tau CE) = ChorEnv.add A x tau (Actor.Map.add B M CE).
+Proof.
+Admitted.
+
+Lemma addadd4 :  forall {X : Type} (CE : ChorEnv.t X) A MA B MB,
+  A <> B -> 
+  Actor.Map.add B MB (Actor.Map.add A MA CE) = Actor.Map.add A MA (Actor.Map.add B MB CE).
+Proof.
+Admitted.
+
+Lemma addadd5 : forall (CE : ChorEnv.t Expr.typ) A x taux B y tauy,
+    Insn.bind_eqb (B, y) (A, x) = false ->
+    (ChorEnv.add A x taux (ChorEnv.add B y tauy CE)) = 
+      (ChorEnv.add B y tauy (ChorEnv.add A x taux CE)).
+Proof.
+Admitted.
+
+(* this lemma may help prove the preceding lemma. *)
+Lemma addadd6 :  forall {X : Type} x taux y tauy (M : Var.Map.t X),
+    x <> y -> 
+    (Var.Map.add y tauy (Var.Map.add x taux M)) =
+      (Var.Map.add x taux (Var.Map.add y tauy M)).
+Proof.
+Admitted.
+
+Lemma addadd7 :  forall (CE : ChorEnv.t Expr.typ) A x tau1 y tau2 M,
+    x <> y -> 
+    Actor.Map.add A (Var.Map.add y tau2 M) (ChorEnv.add A x tau1 CE) =
+      ChorEnv.add A x tau1 (Actor.Map.add A (Var.Map.add y tau2 M) CE).
+Proof.
+Admitted.
+
+Lemma addadd8 :  forall (CE : ChorEnv.t Expr.typ) A x tau M, 
+    Actor.Map.add A (Var.Map.add x tau M) CE =
+      ChorEnv.add A x tau (Actor.Map.add A M CE).
+Proof.
+Admitted.
+
+Lemma nin_mapl : forall (M : Var.Map.t Expr.typ)  x y tau,
+    x <> y ->
+    ~ Var.Map.In x M ->
+    ~ Var.Map.In x (Var.Map.add y tau M).
+Proof.
+Admitted.
+
+Lemma nin_mapr : forall (M : Var.Map.t Expr.typ)  x y tau,
+    x <> y ->
+    ~ Var.Map.In x (Var.Map.add y tau M) ->
+    ~ Var.Map.In x M.
+Proof.
+Admitted.
+
+Lemma nin_nxeq : forall (M : Var.Map.t Expr.typ)  x y tau,
+    ~ Var.Map.In x (Var.Map.add y tau M) -> x <> y.
+Proof.
+Admitted.
+
+(* contrapositive of nin_mapl with mapsto rewrite *)
+Lemma map_in : forall (M : Var.Map.t Expr.typ)  x tau,
+    Var.Map.MapsTo x tau M ->
+    Var.Map.In x M.
+Proof.
+Admitted.
+      
+
+Lemma nin_nbeq : forall (CE : ChorEnv.t Expr.typ) A x tau B y,
+    ~ Var.Map.In y (ChorEnv.find B (ChorEnv.add A x tau CE)) ->
+    Insn.bind_eqb (A, x) (B, y) = false.
+Proof.
+Admitted.
+      
+
+Lemma  contra_nin_nbeq : forall (CE : ChorEnv.t Expr.typ) A x tau B y,
+    Insn.bind_eqb (A, x) (B, y) = true ->
+    Var.Map.In y (ChorEnv.find B (ChorEnv.add A x tau CE)).
+Proof.
+  intros.  
+Admitted.
+
+(* this follows by contraposition of nin_nbeq, atm I am not sure how to
+   prove contrapositive. *)          
+Lemma in_beq : forall (CE : ChorEnv.t Expr.typ) A x tau,
+    Var.Map.In x (ChorEnv.find A (ChorEnv.add A x tau CE)).
+Proof.
+Admitted.
+
+Lemma nin_nbeq_add1 : forall (CE : ChorEnv.t Expr.typ) A x B y tau,
+    Insn.bind_eqb (A, x) (B, y) = false ->
+    ~ Var.Map.In x (ChorEnv.find A CE) ->
+      ~ Var.Map.In x (ChorEnv.find A (ChorEnv.add B y tau CE)).
+Proof.
+Admitted.
+
+Lemma nin_nbeq_add2 : forall (CE : ChorEnv.t Expr.typ) A x B y tau,
+    Insn.bind_eqb (A, x) (B, y) = false ->
+    ~ Var.Map.In x (ChorEnv.find A (ChorEnv.add B y tau CE))->
+    ~ Var.Map.In x (ChorEnv.find A CE).
+Proof.
+Admitted.
+
+
+Lemma ini : forall (Delta : Var.Map.t Expr.typ) Delta1 Delta2 x tau,
+    Var.Map.Partition (Var.Map.add x tau Delta) Delta1 Delta2 ->
+    ~ (Var.Map.In x Delta1) ->
+    (Var.Map.MapsTo x tau Delta2).
+Proof.
+Admitted.
+
+Lemma nin : forall (Delta : Var.Map.t Expr.typ) Delta1' Delta1 Delta2 x tau,
+    Var.Map.add x tau Delta1' = Delta1 ->
+    Var.Map.Partition (Var.Map.add x tau Delta) Delta1 Delta2 ->
+    ~ (Var.Map.In x Delta2) /\ Var.Map.Partition Delta Delta1' Delta2.
+Proof.
+Admitted.
+
+Lemma mapsto_destruct : forall {X : Type} x tau (M : Var.Map.t X) ,
+    Var.Map.MapsTo x tau M ->
+    (exists M', M = Var.Map.add x tau M' /\ ~ Var.Map.In x M').
+Proof.
+Admitted.
+
+Lemma partitioning : forall  {X : Type} (M : Var.Map.t X) M0 M1 M2 M3,
+    Var.Map.Partition M M1 M2 ->
+    Var.Map.Partition M2 M0 M3 ->
+    Var.Map.Partition (Var.Map.concat M1 M0) M1 M0 /\
+      Var.Map.Partition (Var.Map.concat M1 M3) M1 M3 /\      
+      Var.Map.Partition M (Var.Map.concat M1 M0) M3 /\
+      Var.Map.Partition M M0 (Var.Map.concat M1 M3).
+Proof.
+Admitted.
 
 Lemma map_subset_add : forall G1 G2,
     (forall A x (tau : Expr.typ), (ChorEnv.MapsTo A x tau G1 -> ChorEnv.MapsTo A x tau G2)) ->
@@ -288,7 +679,37 @@ Proof.
   intros G1 G2 HMA1 A x tau1 B y tau2 HMA2. 
 Admitted.
 
-(* TODO: Need a stronger statement for weakening---need G' to still be disjoint from D *)
+Lemma add_MapsTo : forall A x (tau : A) m,
+  Var.Map.MapsTo x tau m ->
+  Var.Map.Equal (Var.Map.add x tau m) m.
+Admitted.
+
+(* This is probably redundant. *)
+Lemma no_capture_add : forall A x (tau1 : Expr.typ) I G, 
+    (Insn.rebound_in A x I) = false ->
+    (forall B y tau2, (List.In (B,y) (Insn.bindings I)) ->
+                      ChorEnv.MapsTo A x tau1 G -> ChorEnv.MapsTo A x tau1 (ChorEnv.add B y tau2 G))
+.
+Proof.
+Admitted.
+
+(* STOP Easily(?) proven facts *)
+
+Lemma extension : forall A G x (tau : Expr.typ),
+    ChorEnv.MapsTo A x tau G <-> Var.Map.MapsTo x tau (ChorEnv.find A G).
+Proof.
+  intros A G x tau.
+  split.
+  auto.
+  auto.
+Qed.
+
+Lemma wt_disjoint : forall A G D T C,
+    WellTyped G D T C ->
+    Var.Map.Properties.Disjoint (ChorEnv.find A G) (ChorEnv.find A D).
+Proof.
+Admitted.
+
 Lemma weakening_gen : forall G D T C,
     WellTyped G D T C -> forall G',
       (forall A x tau, ChorEnv.MapsTo A x tau G -> ChorEnv.MapsTo A x tau G') ->
@@ -322,7 +743,7 @@ Proof.
   - intros G' HW. eapply LetBang; eauto.
 
     pose proof (Expr.weakening_gen
-                  e (ChorEnv.find A G) DeltaA1 ThetaA1 (Expr.BANG tau) H (ChorEnv.find A G'))
+                  (ChorEnv.find A G) DeltaA1 ThetaA1 e (Expr.BANG tau) H (ChorEnv.find A G'))
       as HEW.
     apply HEW.
     intros x' tau' HVM.
@@ -338,40 +759,25 @@ Proof.
     auto.
 
   - intros G' HW. eapply LetIn; eauto.
-    pose proof (Expr.weakening_gen e (ChorEnv.find A G) DeltaA1 ThetaA1  tau H (ChorEnv.find A G'))
+    pose proof (Expr.weakening_gen (ChorEnv.find A G) DeltaA1 ThetaA1 e tau H (ChorEnv.find A G'))
       as HEW.
     setoid_rewrite -> extension in HW.
     auto.
 
   - intros G' HW. eapply LetPair; eauto.
-    pose proof (Expr.weakening_gen e (ChorEnv.find A G) DeltaA1 ThetaA1
+    pose proof (Expr.weakening_gen (ChorEnv.find A G) DeltaA1 ThetaA1 e
                   (Expr.Tensor tau1 tau2) H (ChorEnv.find A G'))
       as HEW.
     setoid_rewrite -> extension in HW.
     auto.
 Qed.
 
-Lemma no_capture_add : forall A x (tau1 : Expr.typ) I G, 
-    (Insn.rebound_in A x I) = false ->
-    (forall B y tau2, (List.In (B,y) (Insn.bindings I)) ->
-                      ChorEnv.MapsTo A x tau1 G -> ChorEnv.MapsTo A x tau1 (ChorEnv.add B y tau2 G))
-.
-Proof.
-Admitted.
-
- 
-Lemma add_MapsTo : forall A x (tau : A) m,
-  Var.Map.MapsTo x tau m ->
-  Var.Map.Equal (Var.Map.add x tau m) m.
-Admitted.
-Require Import Setoid.
-
 Lemma wt_subst_bang : forall tau G D T A x v C,
     WellTyped G D T C ->
     Expr.Val v ->
-    Expr.WellTyped (Var.Map.empty _) (Var.Map.empty _) (Var.Map.empty _) v tau ->
+    Expr.WellTyped (Var.Map.empty _) (Var.Map.empty _) (Var.Map.empty _) v (Expr.BANG tau) ->
     ChorEnv.MapsTo A x tau G ->
-    WellTyped G D T (Choreography.subst A x v C).
+               WellTyped G D T (Choreography.subst A x v C).
 Proof.
   intros tau G D T A x v C HWT HV HWTV HA.
   induction HWT.
@@ -387,7 +793,9 @@ Proof.
   
   - eapply Send; eauto.
 
-    + 
+    + (* v must be of the form !e *)
+      inversion HWTV; subst; inversion HV; subst.
+      Var.Map.Tactics.vsimpl.
       destruct (Actor.FSet.MF.eq_dec A A0) eqn:Heq; subst; eauto.
       { (* A = A0 *)
         eapply Expr.wt_subst_bang; eauto.
@@ -472,8 +880,10 @@ Proof.
     + Actor.Map.Tactics.compare A A0; eauto.
     
       {
-        pose proof (Expr.wt_subst_bang e tau (ChorEnv.find A G) DeltaA1 ThetaA1 x v (Expr.Tensor tau1 tau2)) as HEWTS.
-          eapply HEWTS; auto.
+        pose proof (Expr.wt_subst_bang tau (ChorEnv.find A G) DeltaA1 ThetaA1 x v e (Expr.Tensor tau1 tau2)) as HEWTS.
+          eapply HEWTS.
+        { auto. }
+        { apply Expr.weakening; auto. }
         { rewrite add_MapsTo; eauto. }
       }
     + fold Choreography.subst.
@@ -481,6 +891,30 @@ Proof.
         eauto.
 
 Qed.
+
+(* The following lemmas support reasoning in wt_subst_lin *)
+Lemma nri_lin : forall G A x tau D T I C G' D' T',
+    WellTyped G (ChorEnv.add A x tau D) T (I::C) ->
+    WellTyped G' (ChorEnv.add A x tau D') T' C ->
+    ~(Insn.rebound_in A x I = true).
+Proof.
+Admitted.
+
+Lemma esubst_lin : forall Gamma Delta e x v tau,
+    (exists Theta tau', Expr.WellTyped Gamma Delta Theta e tau') -> 
+    ~ Var.Map.In x Gamma -> 
+    (exists Delta', ((Var.Map.add x tau Delta') = Delta) /\
+                      ~(Var.Map.In x Delta'))
+    \/ (~(Var.Map.In x Delta) /\ (Expr.subst x v e) = e).
+Proof.
+Admitted.
+
+Lemma csubst_lin : forall G D T C A x v,
+    WellTyped G D T C ->
+    ~ (Var.Map.In x (ChorEnv.find A D)) ->
+    (Choreography.subst A x v C) = C.
+Proof.
+Admitted.
 
 Lemma wt_subst_lin : forall C ThetaA1 ThetaA2 tau G D T A x v,
     Expr.Val v ->
@@ -491,7 +925,936 @@ Lemma wt_subst_lin : forall C ThetaA1 ThetaA2 tau G D T A x v,
     ~ Var.Map.In x (ChorEnv.find A D) ->
     WellTyped G D T (Choreography.subst A x v C).
 Proof.
-Admitted.
+  intros C. induction C as [| I C IHC ].
+
+  (* Case C = Nil is not possible. *)
+  - intros ThetaA1 ThetaA2 tau G D T A x v Hval Hv HC HinG HinD HninD.
+    inversion HC; subst.
+    pose proof (add_empty_delta A x tau D).
+    contradiction.
+    
+  (* Case C = I::C' *) 
+  - intros ThetaA1 ThetaA2 tau G D T A x v Hval Hv HC HinT HninG HninD.
+    destruct I as [ A' e B y | A' y B z | A' y e | A' y e | A' y z e ].
+
+    (* Case Send *)
+    + inversion HC. subst.
+
+      assert (A = A' \/ A <> A') as HCasesAeqA'.
+      tauto.
+
+      destruct HCasesAeqA' as [HCasesAeqA'L | HCasesAeqA'R].
+
+      (* Case A = A' *)
+      {
+        rewrite <- HCasesAeqA'L in *.
+        
+        assert (HSendety : (exists Theta tau', Expr.WellTyped (ChorEnv.find A G)
+                                                 DeltaA1 Theta e tau')).
+        exists ThetaA0.
+        exists (Expr.BANG tau0).
+        auto.
+        
+        pose proof
+          (esubst_lin (ChorEnv.find A G) DeltaA1 e x v tau HSendety HninG) as HESL.
+        
+        (* Case x in e *) 
+        destruct HESL as [HxinDA | HxninDA].          
+        {
+          (* prepare witness for expression e typing and partioning facts. *)
+          destruct HxinDA as [DeltaA1'].
+          destruct H as [HinDA HninDA'].
+          rewrite <- HinDA in H8.
+          pose proof
+            (Expr.wt_subst e ThetaA1 ThetaA0 tau (ChorEnv.find A G) DeltaA1'
+               (Var.Map.concat ThetaA1 ThetaA0) x v (Expr.BANG tau0)
+               Hval Hv H8) as HWTS.
+          pose proof (find_add A ThetaA2 T) as HFA.
+          rewrite -> HFA in H11.
+          (* partioning facts. *)
+          pose proof
+            (partitioning (ChorEnv.find A T) ThetaA0 ThetaA1 ThetaA2 ThetaA3 HinT H11)
+            as HPartition.
+          destruct HPartition as [HPartitionA [HPartitionB [HPartitionC HPartitionD]]].
+          (* e typing witness. *)
+          specialize (HWTS HPartitionA HninG HninDA').
+          
+          (* prepare witness for choreography C typing *)
+          rewrite -> (addadd1 A D DeltaA2 x tau) in H9.
+          rewrite -> (addadd2 A T ThetaA3 ThetaA2) in H9.
+          
+          (* prepare hypotheses for partitioning requirements *)
+          rewrite -> (add_find D A x tau) in H10.
+          pose proof (nin (ChorEnv.find A D) DeltaA1' DeltaA1 DeltaA2 x tau HinDA H10) as Hnin.
+          pose proof (csubst_lin
+                        (ChorEnv.add B y tau0 G)
+                        (Actor.Map.add A DeltaA2 D)
+                        (Actor.Map.add A ThetaA3 T)
+                        C
+                        A x v H9) as HCSL.
+          rewrite -> (find_add A DeltaA2 D) in HCSL.
+          destruct Hnin as [HninA HninB].
+          
+          (* prove main goal in subcases *)
+          - eapply Send.
+            
+            + auto.
+              
+            + destruct (Actor.FSet.MF.eq_dec A A) eqn:Heq.
+              { eauto. }
+              { contradiction. }
+              
+            + fold Choreography.subst.
+              destruct (Insn.rebound_in A x) eqn:Heq.
+              {
+                assert (~ (Insn.rebound_in A x (Insn.Send A e B y) = true)).
+                simpl.
+                eapply (nbeq A B x y H7).
+                contradiction.
+              }
+              {
+                specialize (HCSL HninA).
+                rewrite -> HCSL.
+                eauto.
+              }
+              
+            + auto.
+              
+            + auto.
+        }
+        (* case x not in e *)
+        {
+          destruct HxninDA as [HxninDAA HxninDAB].
+          rewrite -> (add_find D A x tau) in H10.
+          pose proof (ini (ChorEnv.find A D) DeltaA1 DeltaA2 x tau H10 HxninDAA) as Hini.
+
+          (* partioning facts *)
+          rewrite -> (find_add A ThetaA2 T) in H11.
+          pose proof
+            (partitioning (ChorEnv.find A T) ThetaA0 ThetaA1 ThetaA2 ThetaA3 HinT H11)
+            as HPartition.
+          destruct HPartition as [HPartitionA [HPartitionB [HPartitionC HPartitionD]]].
+          
+          (* prove main goal in subcases *)
+          - eapply Send.
+            
+            + auto.
+              
+            + destruct (Actor.FSet.MF.eq_dec A A) eqn:Heq.
+              {
+                rewrite -> HxninDAB.
+                eauto.
+              }
+              { auto. }
+              
+            + fold Choreography.subst.
+              destruct (Insn.rebound_in A x (Insn.Send A e B y)) eqn:Heq.
+              { 
+                assert (~ (Insn.rebound_in A x (Insn.Send A e B y) = true)).
+                simpl.
+                apply (nbeq A B x y H7).
+                contradiction.
+              }
+              {
+                (* specialize and apply IH *)
+                specialize (IHC ThetaA1 ThetaA3 tau
+                              (ChorEnv.add B y tau0 G)
+                              (Actor.Map.add A (Var.Map.remove x DeltaA2) D)
+                              (Actor.Map.add A (Var.Map.concat ThetaA1 ThetaA3) T)
+                              A x v
+                              Hval Hv).
+                rewrite -> (add_remove D DeltaA2 A x tau) in IHC.
+                rewrite -> (addadd2 A T ThetaA3 (Var.Map.concat ThetaA1 ThetaA3)) in IHC.
+                rewrite -> (addadd1 A D DeltaA2 x tau) in H9.
+                rewrite -> (addadd2 A T ThetaA3 ThetaA2) in H9.
+                specialize (IHC H9).
+                rewrite -> (find_add A (Var.Map.concat ThetaA1 ThetaA3) T) in IHC.
+                specialize (IHC HPartitionB).
+                rewrite -> (find_ab_neq1 A B y tau0 G H7) in IHC.
+                specialize (IHC HninG).
+                rewrite -> (find_add A (Var.Map.remove (elt:=Expr.typ) x DeltaA2) D) in IHC.
+                specialize (IHC (nin_remove DeltaA2 x)).
+                eauto.
+                auto.
+              }
+              
+            + apply (partition_remove (ChorEnv.find A D) DeltaA1 DeltaA2 x tau H10 HninD HxninDAA).
+              
+            + auto.
+        }
+      }
+      (* Case A <> A' *)
+      {
+        - eapply Send.
+
+          + auto.
+
+          + destruct (Actor.FSet.MF.eq_dec A A') eqn:Heq.
+            { contradiction. }
+            { eauto. }
+
+          + fold Choreography.subst.          
+            rewrite -> (addadd3 D A x tau A' DeltaA2) in H9; auto.
+            
+            destruct (Insn.rebound_in A x (Insn.Send A' e B y)) eqn:Heq.
+            {
+              pose proof (nri_lin G A x tau D (Actor.Map.add A ThetaA2 T) (Insn.Send A' e B y) C
+                            (ChorEnv.add B y tau0 G)
+                            (Actor.Map.add A' DeltaA2 D)
+                            (Actor.Map.add A' ThetaA3 (Actor.Map.add A ThetaA2 T))
+                            HC H9) as Hnri.
+              contradiction.
+            }
+            {
+              (* specialize and apply IH *)
+              rewrite -> (addadd4 T A ThetaA2 A' ThetaA3 HCasesAeqA'R) in H9.
+              specialize (IHC ThetaA1 ThetaA2 tau
+                            (ChorEnv.add B y tau0 G)
+                            (Actor.Map.add A' DeltaA2 D)
+                            (Actor.Map.add A' ThetaA3 T)
+                            A x v Hval Hv H9).
+              rewrite -> (find_ab_neq2 A A' ThetaA3 T HCasesAeqA'R) in IHC.
+              rewrite -> (find_ab_neq2 A A' DeltaA2 D HCasesAeqA'R) in IHC.
+              simpl in Heq.
+              pose proof (find_nbeq G A x B y tau0 Heq HninG) as HninG'.
+              eapply (IHC HinT HninG' HninD).
+            }
+
+          + rewrite -> (find_ab_neq1 A' A x tau D) in H10; auto.
+
+          + rewrite -> (find_ab_neq2 A' A ThetaA2 T) in H11; auto.
+      }
+
+    (* Case EPR *)
+    + inversion HC. subst.
+      pose proof (nin_nbeq D A x tau A' y H9) as HninAA'.
+      pose proof (nin_nbeq D A x tau B z H10) as HninAB.
+      rewrite -> (addadd5 D A' y Expr.QUBIT A x tau HninAA') in H8.
+      rewrite -> (addadd5 (ChorEnv.add A' y Expr.QUBIT D) B z Expr.QUBIT A x tau HninAB) in H8.
+      
+      pose proof (nin_nbeq_add1 D A x A' y Expr.QUBIT HninAA' HninD) as HaddAA'.
+      pose proof (nin_nbeq_add1 (ChorEnv.add A' y Expr.QUBIT D) A x B z
+                    Expr.QUBIT HninAB HaddAA') as HaddAB.
+
+      (* specialize and apply IH *)
+      specialize (IHC ThetaA1 ThetaA2 tau G
+                    (ChorEnv.add B z Expr.QUBIT (ChorEnv.add A' y Expr.QUBIT D))
+                    T A x v Hval Hv H8 HinT HninG HaddAB).
+
+      eapply EPR; auto.
+
+      fold Choreography.subst.
+      destruct (Insn.rebound_in A x (Insn.EPR A' y B z)) eqn:Heq.      
+      {
+        simpl in Heq.
+        destruct (Insn.bind_eqb (A, x) (A', y)) eqn:H.
+        {
+          setoid_rewrite -> HninAA' in H.
+          discriminate.
+        }
+        {
+          simpl in Heq.
+          setoid_rewrite -> HninAB in Heq.
+          discriminate.
+        }
+      }
+
+      auto.
+      
+      setoid_rewrite <- (Insn.bind_eqb_symmetric (A', y) (A, x)) in HninAA'.
+      apply (nin_nbeq_add2 D A' y A x tau HninAA') in H9.
+      auto.
+      
+      setoid_rewrite <- (Insn.bind_eqb_symmetric (B, z) (A, x)) in HninAB.
+      apply (nin_nbeq_add2 D B z A x tau HninAB) in H10.
+      auto.
+
+    (* Case Let *)
+    + inversion HC; subst.
+
+      assert (A = A' \/ A <> A') as HCasesAeqA'.
+      tauto.
+
+      destruct HCasesAeqA' as [HCasesAeqA'L | HCasesAeqA'R].
+
+      (* Case A = A' *)
+      {
+        rewrite <- HCasesAeqA'L in *.
+        
+        assert (HSendety : (exists Theta tau', Expr.WellTyped (ChorEnv.find A G) DeltaA1 Theta e tau')).
+        exists ThetaA0.
+        exists tau0.
+        auto.
+        
+        pose proof
+          (esubst_lin (ChorEnv.find A G) DeltaA1 e x v tau HSendety HninG) as HESL.
+      
+        (* Case x in e *) 
+        destruct HESL as [HxinDA | HxninDA].          
+        {
+          (* prepare witness for expression e typing and partioning facts. *)
+          destruct HxinDA as [DeltaA1'].
+          destruct H as [HinDA HninDA'].
+          rewrite <- HinDA in H3.
+          pose proof
+            (Expr.wt_subst e ThetaA1 ThetaA0 tau (ChorEnv.find A G) DeltaA1'
+               (Var.Map.concat ThetaA1 ThetaA0) x v tau0
+               Hval Hv H3) as HWTS.
+          pose proof (find_add A ThetaA2 T) as HFA.
+          rewrite -> HFA in H9.
+          (* partioning facts. *)
+          pose proof
+            (partitioning (ChorEnv.find A T) ThetaA0 ThetaA1 ThetaA2 ThetaA3 HinT H9)
+            as HPartition.
+          destruct HPartition as [HPartitionA [HPartitionB [HPartitionC HPartitionD]]].
+          (* e typing witness. *)
+          specialize (HWTS HPartitionA HninG HninDA').
+
+          (* prepare witness for choreography C typing *)
+          rewrite -> (addadd1 A D (Var.Map.add y tau0 DeltaA2) x tau) in H7. 
+          rewrite -> (addadd2 A T ThetaA3 ThetaA2) in H7.
+
+          (* prepare hypotheses for partitioning requirements *)
+          rewrite -> (add_find D A x tau) in H8.
+          pose proof (nin (ChorEnv.find A D) DeltaA1' DeltaA1 DeltaA2 x tau HinDA H8) as Hnin.
+          pose proof (csubst_lin
+                        G
+                        (Actor.Map.add A  (Var.Map.add y tau0 DeltaA2) D)
+                        (Actor.Map.add A ThetaA3 T)
+                        C
+                        A x v H7) as HCSL.
+          rewrite -> (find_add A (Var.Map.add y tau0 DeltaA2) D) in HCSL.
+          destruct Hnin as [HninA HninB].
+
+          (* prove main goal in subcases *)
+          - eapply LetIn.
+            
+            + destruct (Actor.FSet.MF.eq_dec A A) eqn:Heq.
+              { eauto. }
+              { contradiction. }
+              
+            + fold Choreography.subst.
+              destruct (Insn.rebound_in A x) eqn:Heq.
+              {
+                eauto.
+              }
+              {
+                unfold Insn.rebound_in in Heq.
+                specialize (HCSL (nin_mapl DeltaA2 x y tau0 (nbeqeq A x y Heq) HninA)).
+                rewrite -> HCSL.
+                eauto.
+              }
+              
+            + auto.
+              
+            + auto.
+
+            + auto.
+        }
+        (* case x not in e *)
+        {
+          destruct HxninDA as [HxninDAA HxninDAB].
+          rewrite -> (add_find D A x tau) in H8.
+          pose proof (ini (ChorEnv.find A D) DeltaA1 DeltaA2 x tau H8 HxninDAA) as Hini.
+
+          (* (de)construct environment for typing C *)
+          pose proof (mapsto_destruct x tau DeltaA2 Hini) as HDA2.
+          destruct HDA2 as [DeltaA2'].
+          destruct H as [HDA2A HDA2B].
+
+          (* partioning facts. *)
+          rewrite -> (find_add A ThetaA2 T) in H9.
+          pose proof
+            (partitioning (ChorEnv.find A T) ThetaA0 ThetaA1 ThetaA2 ThetaA3 HinT H9) 
+            as HPartition.                
+          destruct HPartition as [HPartitionA [HPartitionB [HPartitionC HPartitionD]]].
+          
+          (* prove main goal in subcases *)
+          - eapply LetIn.
+            
+            + destruct (Actor.FSet.MF.eq_dec A A) eqn:Heq.
+              {
+                rewrite -> HxninDAB.
+                eauto.
+              }
+              { auto. }
+
+            + fold Choreography.subst.
+              destruct (Insn.rebound_in A x (Insn.Let A y e)) eqn:Heq.
+              (* impossible case x = y *)
+              {
+                (* Note to ces: This case is provable constructively as follows, but instantiates
+                   existential variables that falsify the hypotheses for subsequent case. *)
+                (*
+                  rewrite -> (addadd1 A D (Var.Map.add y tau0 DeltaA2) x tau) in H7.
+                  rewrite -> (addadd2 A T ThetaA3 ThetaA2) in H7.
+                  eauto.
+                 *)
+                pose proof (beqeq A x y Heq).
+                pose proof (map_in DeltaA2 x tau Hini).
+                rewrite <- H in H10.
+                contradiction.
+              }
+              (* case x <> y *)
+              {
+                (* prepare C typing. *)
+                rewrite -> (addadd1 A D (Var.Map.add y tau0 DeltaA2) x tau) in H7.
+                rewrite -> HDA2A in H7.
+                rewrite -> (addadd6 x tau y tau0 DeltaA2') in H7.
+                rewrite -> (addadd2 A T ThetaA3 ThetaA2) in H7.
+                
+                               
+                (* specialize and apply IH. *)
+                specialize (IHC ThetaA1 ThetaA3 tau
+                              G
+                              (Actor.Map.add A (Var.Map.add y tau0 DeltaA2') D)
+                              (Actor.Map.add A (Var.Map.concat ThetaA1 ThetaA3) T)
+                              A x v Hval Hv).
+                
+                unfold ChorEnv.add in IHC.
+                rewrite -> (find_add A (Var.Map.add y tau0 DeltaA2') D) in IHC.
+                rewrite -> (addadd2 A D (Var.Map.add x tau (Var.Map.add y tau0 DeltaA2'))) in IHC.
+                rewrite -> (addadd2 A T ThetaA3 (Var.Map.concat ThetaA1 ThetaA3)) in IHC.
+                specialize (IHC H7).
+
+                unfold Insn.rebound_in in Heq.
+                rewrite -> (find_add A (Var.Map.concat ThetaA1 ThetaA3) T) in IHC.
+                specialize (IHC HPartitionB HninG
+                              (nin_mapl DeltaA2' x y tau0 (nbeqeq A x y Heq) HDA2B)).                
+
+                eauto.
+
+                apply (nbeqeq A x y Heq).
+              }
+              
+            + pose proof (partition_remove (ChorEnv.find A D) DeltaA1 DeltaA2 x tau
+                            H8 HninD HxninDAA).
+              rewrite -> (remove_add x tau DeltaA2' DeltaA2 HDA2B HDA2A) in H.
+              auto.
+
+            + auto.
+
+            + rewrite -> HDA2A in H10.
+              pose proof (nin_mapr DeltaA2' y x tau (nin_nxeq DeltaA2' y x tau H10) H10).
+              auto.
+        }
+      }
+      (* Case A <> A' *)
+      {
+        - eapply LetIn.
+          
+          + destruct (Actor.FSet.MF.eq_dec A A') eqn:Heq.
+            { contradiction. }
+            { eauto. } 
+            
+          + fold Choreography.subst.
+            destruct (Insn.rebound_in A x (Insn.Let A' y e)) eqn:Heq.
+            {
+              unfold Insn.rebound_in in Heq.
+              pose proof (beq A A' x y).
+              destruct H.
+              specialize (H Heq).
+              destruct H.
+              contradiction.
+            }
+            {
+              (* prepare C typing *)
+              rewrite -> (addadd3 D A x tau A' (Var.Map.add y tau0 DeltaA2) HCasesAeqA'R) in H7.
+              rewrite -> (addadd4 T A ThetaA2 A' ThetaA3 HCasesAeqA'R) in H7.
+              
+              (* specialize and apply IH *)
+              specialize (IHC ThetaA1 ThetaA2 tau G
+                            (Actor.Map.add A' (Var.Map.add y tau0 DeltaA2) D)
+                            (Actor.Map.add A' ThetaA3 T)
+                            A x v Hval Hv H7).
+ 
+              rewrite -> (find_ab_neq2 A A' ThetaA3 T HCasesAeqA'R) in IHC.
+              rewrite -> (find_ab_neq2 A A' (Var.Map.add y tau0 DeltaA2) D HCasesAeqA'R) in IHC.
+
+              specialize (IHC HinT HninG HninD).
+              eauto.
+            }
+
+            + assert (A' <> A).
+              auto.
+              rewrite -> (find_ab_neq1 A' A x tau D H) in H8.
+              auto.
+
+            + assert (A' <> A).
+              auto.
+              rewrite -> (find_ab_neq2 A' A ThetaA2 T H) in H9.
+              auto.
+
+            + auto.
+      }
+
+    (* Case LetBang *)
+    + inversion HC; subst.
+
+      assert (A = A' \/ A <> A') as HCasesAeqA'.
+      tauto.
+
+      destruct HCasesAeqA' as [HCasesAeqA'L | HCasesAeqA'R].
+
+      (* Case A = A' *)
+      {
+        rewrite <- HCasesAeqA'L in *.
+
+        rewrite -> (addadd1 A D DeltaA2 x tau) in H7.
+        rewrite -> (addadd2 A T ThetaA3 ThetaA2) in H7.
+        
+        assert (HSendety : (exists Theta tau', Expr.WellTyped (ChorEnv.find A G)
+                                                 DeltaA1 Theta e tau')).
+        exists ThetaA0.
+        exists (Expr.BANG tau0).
+        auto.
+        
+        pose proof
+          (esubst_lin (ChorEnv.find A G) DeltaA1 e x v tau HSendety HninG) as HESL.
+        
+        (* Case x in e *) 
+        destruct HESL as [HxinDA | HxninDA].          
+        {
+          (* prepare witness for expression e typing and partioning facts. *)
+          destruct HxinDA as [DeltaA1'].
+          destruct H as [HinDA HninDA'].
+
+          (* expression typing *)
+          rewrite <- HinDA in H6.
+          
+          (* partioning facts. *)
+          rewrite -> (find_add A ThetaA2 T) in H9.
+          pose proof
+            (partitioning (ChorEnv.find A T) ThetaA0 ThetaA1 ThetaA2 ThetaA3 HinT H9)
+            as HPartition.
+          destruct HPartition as [HPartitionA [HPartitionB [HPartitionC HPartitionD]]].
+          rewrite -> (add_find D A x tau) in H8.
+          pose proof (nin (ChorEnv.find A D) DeltaA1' DeltaA1 DeltaA2 x tau HinDA H8) as Hnin.
+          destruct Hnin as [HninA HninB].
+               
+          eapply LetBang.
+          
+          + destruct (Actor.FSet.MF.eq_dec A A) eqn:Heq.
+            {
+            
+              pose proof
+                (Expr.wt_subst e ThetaA1 ThetaA0 tau (ChorEnv.find A G) DeltaA1'
+                   (Var.Map.concat ThetaA1 ThetaA0) x v (Expr.BANG tau0)
+                   Hval Hv H6 HPartitionA HninG HninDA') as HWTS.
+              eauto.
+            }
+            {
+              contradiction.
+            }
+
+          +  fold Choreography.subst.
+             destruct (Insn.rebound_in A x) eqn:Heq.
+             { eauto.}
+             {
+               pose proof (csubst_lin
+                             (ChorEnv.add A y tau0 G)
+                             (Actor.Map.add A DeltaA2 D)
+                             (Actor.Map.add A ThetaA3 T)
+                             C
+                             A x v H7) as HCSL.
+               rewrite -> (find_add A DeltaA2 D) in HCSL.
+                       
+               specialize (HCSL HninA).
+               rewrite -> HCSL.
+               eauto.
+             }
+             
+          + auto.
+
+          + auto.
+        }
+        (* case x not in e *)
+        {
+          destruct HxninDA as [HxninDAA HxninDAB].
+          rewrite -> (add_find D A x tau) in H8.
+          pose proof (ini (ChorEnv.find A D) DeltaA1 DeltaA2 x tau H8 HxninDAA) as Hini.
+
+          
+          (* (de)construct environment for typing C *)
+          pose proof (mapsto_destruct x tau DeltaA2 Hini) as HDA2.
+          destruct HDA2 as [DeltaA2'].
+          destruct H as [HDA2A HDA2B].
+          
+          (* partioning facts. *)
+          rewrite -> (find_add A ThetaA2 T) in H9.
+          pose proof
+            (partitioning (ChorEnv.find A T) ThetaA0 ThetaA1 ThetaA2 ThetaA3 HinT H9)
+            as HPartition.
+          destruct HPartition as [HPartitionA [HPartitionB [HPartitionC HPartitionD]]].
+          
+          (* prove main goal in subcases *)
+          - eapply LetBang.
+            
+            + destruct (Actor.FSet.MF.eq_dec A A) eqn:Heq.
+              {
+                rewrite -> HxninDAB.
+                eauto.
+              }
+              { auto. }
+              
+            + fold Choreography.subst.
+              (* impossible case due to env disjointness *)
+              destruct (Insn.rebound_in A x (Insn.LetBang A y e)) eqn:Heq.
+              {
+                unfold Insn.rebound_in in Heq.
+                pose proof (beqeq A x y Heq).
+                rewrite <- H in *.
+
+                pose proof (wt_disjoint A (ChorEnv.add A x tau0 G) (Actor.Map.add A DeltaA2 D)
+                              (Actor.Map.add A ThetaA3 T) C H7) as Hwtdj.
+                rewrite (find_add A DeltaA2 D) in Hwtdj.
+
+                (* This does not go through with tauto. 
+                   pose proof (nin_nbeq G A x tau0 A x).
+                   assert (Insn.bind_eqb (A, x) (A, x) = true ->
+                       Var.Map.In (elt:=Expr.typ) x (ChorEnv.find A (ChorEnv.add A x tau0 G))).
+                   tauto. *)
+
+                pose proof (nin_dj x (ChorEnv.find A (ChorEnv.add A x tau0 G)) DeltaA2
+                              Hwtdj (map_in DeltaA2 x tau Hini)) as Hcontra1.
+                pose proof (in_beq G A x tau0) as Hcontra2.
+                contradiction.
+              }
+              {          
+                rewrite -> HDA2A in H7.
+                rewrite -> (addadd8 D A x tau DeltaA2') in H7.
+
+                (* specialize and apply IH *)
+                specialize (IHC ThetaA1 ThetaA3 tau
+                              (ChorEnv.add A' y tau0 G)
+                              (Actor.Map.add A DeltaA2' D)
+                              (Actor.Map.add A (Var.Map.concat ThetaA1 ThetaA3) T)
+                              A x v
+                              Hval Hv).
+
+                rewrite <- HCasesAeqA'L in IHC.
+                rewrite -> (addadd2 A T ThetaA3 (Var.Map.concat ThetaA1 ThetaA3)) in IHC.
+                rewrite -> (find_add A (Var.Map.concat ThetaA1 ThetaA3) T) in IHC.
+                rewrite -> (find_add A DeltaA2' D) in IHC.
+                pose proof (nin_nbeq_add1 G A x A y tau0 Heq HninG) as HninGy.
+                
+                specialize (IHC H7 HPartitionB HninGy HDA2B).
+
+                eauto.
+              }
+
+            +  assert (Var.Map.add x tau DeltaA2' = DeltaA2) as Hdel; auto.
+               pose proof (partitionm_refl (Var.Map.add x tau (ChorEnv.find A D)) DeltaA1 DeltaA2 H8) as Hpart.
+               pose proof (nin (ChorEnv.find A D) DeltaA2' DeltaA2 DeltaA1 x tau Hdel Hpart) as Hnin.
+               destruct Hnin as [HninA HninB].
+               pose proof (partitionm_refl (ChorEnv.find A D) DeltaA2' DeltaA1 HninB).
+               auto.
+
+            + auto.
+        }
+      }
+      (* Case A <> A' *)
+      {
+        - eapply LetBang.
+          
+          + destruct (Actor.FSet.MF.eq_dec A A') eqn:Heq.
+            { contradiction. }
+            { eauto. } 
+            
+          + fold Choreography.subst.
+            destruct (Insn.rebound_in A x (Insn.LetBang A' y e)) eqn:Heq.
+            {
+              unfold Insn.rebound_in in Heq.
+              pose proof (beq A A' x y).
+              destruct H.
+              specialize (H Heq).
+              destruct H.
+              contradiction.
+            }
+            {
+              (* prepare C typing *)
+              rewrite -> (addadd4 T A ThetaA2 A' ThetaA3 HCasesAeqA'R) in H7.
+              rewrite -> (addadd3 D A x tau A' DeltaA2 HCasesAeqA'R) in H7.
+
+              (* specialize and apply IH *)
+              specialize (IHC ThetaA1 ThetaA2 tau
+                            (ChorEnv.add A' y tau0 G)
+                            (Actor.Map.add A' DeltaA2 D)
+                            (Actor.Map.add A' ThetaA3 T)
+                            A x v Hval Hv H7).
+              rewrite -> (find_ab_neq2 A A' ThetaA3 T HCasesAeqA'R) in IHC.
+              rewrite -> (find_ab_neq2 A A' DeltaA2 D HCasesAeqA'R) in IHC.
+              simpl in Heq.
+              pose proof (find_nbeq G A x A' y tau0 Heq HninG) as HninG'.
+              eapply (IHC HinT HninG' HninD).
+            }
+
+            + assert (A' <> A).
+              auto.
+              rewrite -> (find_ab_neq1 A' A x tau D H) in H8.
+              auto.
+
+            + assert (A' <> A).
+              auto.
+              rewrite -> (find_ab_neq2 A' A ThetaA2 T H) in H9.
+              auto.
+      }
+
+      (* Case LetPair *)
+    + inversion HC; subst.
+
+      assert (A = A' \/ A <> A') as HCasesAeqA'.
+      tauto.
+
+      destruct HCasesAeqA' as [HCasesAeqA'L | HCasesAeqA'R].
+
+      (* Case A = A' *)
+      {
+        rewrite <- HCasesAeqA'L in *.
+
+        rewrite -> (addadd1 A D (Var.Map.add y tau1 (Var.Map.add z tau2 DeltaA2)) x tau) in H8.
+        rewrite -> (addadd2 A T ThetaA3 ThetaA2) in H8.
+        
+        assert (HSendety : (exists Theta tau', Expr.WellTyped (ChorEnv.find A G)
+                                                 DeltaA1 Theta e tau')).
+        exists ThetaA0.
+        exists (Expr.Tensor tau1 tau2).
+        auto. 
+        
+        pose proof
+          (esubst_lin (ChorEnv.find A G) DeltaA1 e x v tau HSendety HninG) as HESL.
+
+        (* Case x in e *) 
+        destruct HESL as [HxinDA | HxninDA].          
+        {
+          (* prepare witness for expression e typing and partioning facts. *)
+          destruct HxinDA as [DeltaA1'].
+          destruct H as [HinDA HninDA'].
+          rewrite <- HinDA in H4.
+          pose proof
+            (Expr.wt_subst e ThetaA1 ThetaA0 tau (ChorEnv.find A G) DeltaA1'
+               (Var.Map.concat ThetaA1 ThetaA0) x v (Expr.Tensor tau1 tau2)
+               Hval Hv H4) as HWTS.
+          pose proof (find_add A ThetaA2 T) as HFA.
+          rewrite -> HFA in H10.
+          (* partioning facts. *)
+          pose proof
+            (partitioning (ChorEnv.find A T) ThetaA0 ThetaA1 ThetaA2 ThetaA3 HinT H10)
+            as HPartition.
+          destruct HPartition as [HPartitionA [HPartitionB [HPartitionC HPartitionD]]].
+          (* e typing witness. *)
+          specialize (HWTS HPartitionA HninG HninDA').
+
+          (* prepare hypotheses for partitioning requirements *)
+          rewrite -> (add_find D A x tau) in H9.
+          pose proof (nin (ChorEnv.find A D) DeltaA1' DeltaA1 DeltaA2 x tau HinDA H9) as Hnin.
+          pose proof (csubst_lin
+                        G
+                        (Actor.Map.add A (Var.Map.add y tau1 (Var.Map.add z tau2 DeltaA2)) D)
+                        (Actor.Map.add A ThetaA3 T)
+                        C
+                        A x v H8) as HCSL.
+          rewrite -> (find_add A (Var.Map.add y tau1 (Var.Map.add z tau2 DeltaA2)) D) in HCSL.
+          destruct Hnin as [HninA HninB].
+
+          (* prove main goal in subcases *)
+          - eapply LetPair.
+            
+            + destruct (Actor.FSet.MF.eq_dec A A) eqn:Heq.
+              { eauto. }
+              { contradiction. }
+              
+            + fold Choreography.subst.
+              destruct (Insn.rebound_in A x) eqn:Heq.
+              {
+                eauto.
+              }
+              {
+                unfold Insn.rebound_in in Heq.
+
+                (* NOTE: nice boolean eq rewrite Lemma from Bool.Bool *)
+                rewrite orb_false_iff in Heq.
+                destruct Heq as [HeqA HeqB].
+                
+                pose proof (nin_mapl DeltaA2 x z tau2 (nbeqeq A x z HeqB) HninA) as Hninz.
+                specialize (HCSL (nin_mapl (Var.Map.add z tau2 DeltaA2)
+                                    x y tau1 (nbeqeq A x y HeqA) Hninz)).
+                rewrite -> HCSL.
+                eauto.
+              }
+              
+            + auto.
+              
+            + auto.
+
+            + auto.
+
+            + auto.
+        }
+        (* case x not in e *)
+        {
+          destruct HxninDA as [HxninDAA HxninDAB].
+          rewrite -> (add_find D A x tau) in H9.
+          pose proof (ini (ChorEnv.find A D) DeltaA1 DeltaA2 x tau H9 HxninDAA) as Hini.
+
+          (* (de)construct environment for typing C *)
+          pose proof (mapsto_destruct x tau DeltaA2 Hini) as HDA2.
+          destruct HDA2 as [DeltaA2'].
+          destruct H as [HDA2A HDA2B].
+
+          (* partioning facts. *)
+          rewrite -> (find_add A ThetaA2 T) in H10.
+          pose proof
+            (partitioning (ChorEnv.find A T) ThetaA0 ThetaA1 ThetaA2 ThetaA3 HinT H10) 
+            as HPartition.                
+          destruct HPartition as [HPartitionA [HPartitionB [HPartitionC HPartitionD]]].
+          
+          (* prove main goal in subcases *)
+          - eapply LetPair.
+            
+            + destruct (Actor.FSet.MF.eq_dec A A) eqn:Heq.
+              {
+                rewrite -> HxninDAB.
+                eauto.
+              }
+              { auto. }
+
+            + fold Choreography.subst.
+              destruct (Insn.rebound_in A x (Insn.LetPair A y z e)) eqn:Heq.
+              (* impossible case x = y *)
+              {
+                unfold Insn.rebound_in in Heq.
+
+                (* NOTE: nice boolean eq rewrite Lemma from Bool.Bool *)
+                rewrite orb_true_iff in Heq.
+                destruct Heq as [HeqA | HeqB].
+                {
+                  pose proof (beqeq A x y HeqA).
+                  rewrite <- H in *.
+                  pose proof (map_in DeltaA2 x tau Hini).
+                  contradiction.
+                }
+                {
+                  pose proof (beqeq A x z HeqB).
+                  pose proof (map_in DeltaA2 x tau Hini).
+                  rewrite <- H in H12.
+                  contradiction.
+                }
+              }
+              (* case x <> y,z *)
+              {
+                unfold Insn.rebound_in in Heq.
+                rewrite orb_false_iff in Heq.
+                destruct Heq as [HeqA HeqB].
+                pose proof (nbeqeq A x y HeqA).
+                pose proof (nbeqeq A x z HeqB).
+                
+                (* prepare C typing. *)
+                rewrite -> HDA2A in H8.                
+                rewrite -> (addadd6 x tau z tau2 DeltaA2' H0) in H8.
+                rewrite -> (addadd6 x tau y tau1 (Var.Map.add z tau2 DeltaA2') H) in H8.
+                rewrite -> (addadd8 D A x tau (Var.Map.add y tau1 (Var.Map.add z tau2 DeltaA2'))) in H8.
+
+                specialize (IHC ThetaA1 ThetaA3 tau
+                              G
+                              (Actor.Map.add A (Var.Map.add y tau1 (Var.Map.add z tau2 DeltaA2')) D)
+                              (Actor.Map.add A (Var.Map.concat ThetaA1 ThetaA3) T)
+                              A x v Hval Hv).
+
+                rewrite -> (addadd2 A T ThetaA3 (Var.Map.concat ThetaA1 ThetaA3)) in IHC.
+                rewrite -> (find_add A (Var.Map.concat ThetaA1 ThetaA3) T) in IHC.
+                rewrite -> (find_add A (Var.Map.add y tau1 (Var.Map.add z tau2 DeltaA2')) D) in IHC.
+
+               
+                pose proof (nin_mapl DeltaA2' x z tau2 H0 HDA2B) as Hninz.
+                pose proof (nin_mapl (Var.Map.add z tau2 DeltaA2') x y tau1 H Hninz) as Hniny.
+                
+                specialize (IHC H8 HPartitionB HninG Hniny).
+                eauto.
+              }
+
+            + pose proof (partition_remove (ChorEnv.find A D) DeltaA1 DeltaA2 x tau
+                            H9 HninD HxninDAA).
+              rewrite -> (remove_add x tau DeltaA2' DeltaA2 HDA2B HDA2A) in H.
+              auto.
+
+            + auto.
+
+            + rewrite -> HDA2A in H11.
+              pose proof (nin_mapr DeltaA2' y x tau (nin_nxeq DeltaA2' y x tau H11) H11).
+              auto.
+
+            + rewrite -> HDA2A in H12.
+              pose proof (nin_mapr DeltaA2' z x tau (nin_nxeq DeltaA2' z x tau H12) H12).
+              auto.
+        }
+      }
+      (* Case A <> A' *)
+      {
+        - eapply LetPair.
+
+          + destruct (Actor.FSet.MF.eq_dec A A') eqn:Heq.
+            { contradiction. }
+            { eauto. } 
+
+          + fold Choreography.subst.
+            destruct (Insn.rebound_in A x (Insn.LetPair A' y z e)) eqn:Heq.
+            {
+              unfold Insn.rebound_in in Heq.
+              rewrite orb_true_iff in Heq.
+              destruct Heq as [Heqxy | Heqxz].
+              {
+                pose proof (beq A A' x y).
+                destruct H as [HA HB].
+                specialize (HA Heqxy).
+                destruct HA.
+                contradiction.
+              }
+              {
+                pose proof (beq A A' x z).
+                destruct H as [HA HB].
+                specialize (HA Heqxz).
+                destruct HA.
+                contradiction.
+              }
+            }
+            { 
+              (* prepare C typing *)
+              Check addadd3.
+              Check addadd4.
+              rewrite -> (addadd3 D A x tau A'
+                            (Var.Map.add y tau1 (Var.Map.add z tau2 DeltaA2)) HCasesAeqA'R) in H8.
+              rewrite -> (addadd4 T A ThetaA2 A' ThetaA3 HCasesAeqA'R) in H8.
+              
+              (* specialize and apply IH *)
+              specialize (IHC ThetaA1 ThetaA2 tau G
+                            (Actor.Map.add A' (Var.Map.add y tau1 (Var.Map.add z tau2 DeltaA2)) D)
+                            (Actor.Map.add A' ThetaA3 T)
+                            A x v Hval Hv H8).
+ 
+              rewrite -> (find_ab_neq2 A A' ThetaA3 T HCasesAeqA'R) in IHC.
+              rewrite -> (find_ab_neq2 A A' (Var.Map.add y tau1 (Var.Map.add z tau2 DeltaA2))
+                            D HCasesAeqA'R) in IHC.
+
+              specialize (IHC HinT HninG HninD).
+              eauto.
+            }
+
+          + assert (A' <> A).
+            auto.
+            rewrite -> (find_ab_neq1 A' A x tau D H) in H9.
+            auto.
+            
+          + assert (A' <> A).
+            auto.
+            rewrite -> (find_ab_neq2 A' A ThetaA2 T H) in H10.
+            auto.
+            
+          + auto.
+
+          + auto.
+      }
+Qed.
 
     
 (* placeholder for well-formedness definition *)
